coq/Logic/ZF/Difference.v
@@ -2,7 +2,7 @@ Declare Scope ZF_Difference_scope.
 Open    Scope ZF_Difference_scope.
 
 Require Import Logic.ZF.Core.
-Require Import Logic.ZF.Comprehension.
+Require Import Logic.ZF.Specification.
 
 (* The set a \ b is made of those elements of a which do not belong to b.       *)
 Definition difference (a b:U) : U := :{a | fun x => ~ x :< b }:.
@@ -13,5 +13,5 @@ Notation "a :\: b" := (difference a b)
 Proposition DiffCharac : forall (a b:U),
   forall x, x :< a:\:b <-> x :< a /\ ~ x :< b.
 Proof.
-  intros a b x. unfold difference. apply CompCharac.
+  intros a b x. unfold difference. apply SpecCharac.
 Qed.
